stlc_unary.v
@@ -43,17 +43,7 @@ Proof.
   intros.
   exists v.
   intuition.
-  - constructor.
-  - eauto using V_value.
-Qed.
-
-Lemma has_type_wf :
-  forall G e ty,
-    has_type.t G e ty ->
-    expr.wf (List.length G) e.
-Proof.
-  induction 1; simpl in *; intuition.
-  pose proof nth_error_Some G x. intuition congruence.
+  eauto using V_value.
 Qed.
 
 Lemma V_closed :
@@ -68,15 +58,13 @@ Qed.
 Lemma V_list_closed :
   forall G vs,
     Forall2 V G vs ->
-    Forall (expr.wf 1) (expr.var 0 :: map (expr.shift 0 1) vs).
+    Forall (expr.wf 0) vs.
 Proof.
   intros G vs F.
-  constructor.
-  - simpl. omega.
-  - rewrite Forall_map.
-    induction F; constructor; auto.
-    apply expr.wf_shift with (d := 1) (n := 0).
-    now eauto using V_closed.
+  apply Forall_from_nth.
+  intros n e NEe.
+  destruct (Forall2_nth_error_l F NEe) as [ty [NEty Ve]].
+  eauto using V_closed.
 Qed.
 
 Lemma E_step :
@@ -88,9 +76,7 @@ Proof.
   intros ty e e' S HE.
   revert ty HE.
   induction S; intros ty0 [v [Star [Val HV]]]; exists v; intuition.
-  - eapply step.step_l; eauto.
-  - eapply step.step_l; eauto.
-  - eapply step.step_l; eauto.
+  all: eapply step.step_l; eauto.
 Qed.
 
 Lemma E_star :
@@ -114,58 +100,36 @@ Proof.
   induction 1; intros vs F.
   - cbn [expr.subst].
     destruct (Forall2_nth_error_r F H) as [v [Hvs HV]].
+    simpl.
     rewrite Hvs.
     auto using V_E.
   - apply V_E.
     reflexivity.
-  - cbn [expr.subst].
-    apply V_E.
+  - apply V_E.
     cbn [V].
+    assert (expr.wf (S (length vs)) e) as WFe
+      by (apply has_type.wf in H;
+          simpl in *;
+          now erewrite Forall2_length in * by eauto).
     split.
-    + simpl. apply expr.wf_subst.
-      * simpl. rewrite map_length.
-        apply has_type_wf in H.
-        simpl in *.
-        now erewrite Forall2_length in * by eauto.
-      * eapply V_list_closed; eauto.
-    + eexists. split. reflexivity.
+    + apply expr.wf_subst; eauto using V_list_closed.
+    + exists (expr.subst (expr.descend 1 vs) e).
+      split; [now rewrite expr.descend_1|].
       intros e2 Ve2.
-      cbn [expr.subst].
-      set (vs' := e2 :: vs).
-      match goal with
-      | [  |- E _ ?foo ] =>
-        replace foo with (expr.subst vs' e)
-      end.
-      apply IHt.
-      constructor; auto.
-      rewrite expr.subst_subst.
-      * simpl. f_equal. subst vs'. f_equal.
-        rewrite map_map.
-        erewrite map_ext_in; [now rewrite map_id|].
-        intros e' I. simpl.
-        rewrite expr.subst_shift_singleton; auto.
-        destruct (In_nth_error _ _ I) as [n NE].
-        destruct (Forall2_nth_error_l F NE) as [ty [NE2 HV]].
-        now eauto using V_closed.
-      * simpl. rewrite map_length.
-        eapply has_type_wf in H. simpl in *.
-        now erewrite <- Forall2_length by eauto.
-      * eapply V_list_closed; eauto.
-  - simpl.
+      rewrite expr.subst_cons; eauto using V_list_closed.
+  - cbn [expr.subst].
     specialize (IHt1 vs F).
     specialize (IHt2 vs F).
     destruct IHt1 as [v1 [S1 [Val1 V1]]].
     destruct IHt2 as [v2 [S2 [Val2 V2]]].
     destruct V1 as [WF1 [body [? H1]]].
     subst v1.
-    apply E_star with (e' := expr.subst [v2] body); [|now eauto].
+    eapply E_star; [|now eauto].
     eapply step.star_trans.
-    eapply step.star_app1; eauto.
+    eapply step.star_app1. now eauto.
     eapply step.star_trans.
-    eapply step.star_app2; eauto.
-    eapply step.step_l.
-    apply step.beta.
-    constructor.
+    eapply step.star_app2. now eauto.
+    eauto using step.step_l, step.beta.
 Qed.
 Print Assumptions fundamental.
 
